:wrench: modify part3

part3.dfy
@@ -1,26 +1,30 @@
 /*
-  Part 2: Design by Contract
+  Part 3: Loop invariants
 
-  In this part, we will give you the pre/postconditions
+  The last part consists of 5 loop invariant problems.
+
+  This part is written in a "design by contract" style:
+  we will give you the pre/postconditions
   for several methods. Your job is to implement the
-  function so that the verification passes.
+  method so that the verification passes.
 
   Requirements:
+  - Every method that you implement should have a `while` loop!
+    If you find a way to do it without a loop, you may explain
+    it in a comment, but please implement it with a loop.
+
+  - Don't change the method signatures or pre/postconditions
+    for any of the methods!
+    You can always add helper methods if needed.
+
   - Since the specs are already written, the only requirement
     is that you implement the methods so that the specs pass.
 
-  - Don't change the function signatures or pre/postconditions
-    for any of the methods. You can add helper functions if needed.
-
-  - You will need to use loop invariants for 1 and 2.
-
-  - Your code should pass the Dafny verifier:
-      dafny verify part2.dfy
-    should pass with no errors or warnings.
-
-    You can also simply check that the green bar shows up next
-    to every function in VSCode, throughout the whole file,
-    with no errors (shown in red).
+  - Your file should pass the Dafny verifier with no errors or warnings.
+    Look for the green bars or (if you have the command line):
+    ```
+    Dafny program verifier finished with <n> verified, 0 errors
+    ```
 */
 
 /*
@@ -65,37 +69,18 @@ method NumDigits(n: int) returns (digits: int)
 }
 
 /*
-  3. Function to increment a stopwatch
+  3. List copy
 
-  The last function assumes that we have a stopwatch that
-  stores the time as a number of seconds, minutes, hours, and days.
-
-  The function AdvanceStopwatch increments the stopwatch by a given
-  number of seconds, and returns the new values.
+  Copy a list (sequence) into a new sequence.
+  For example, if the input list is
+    [1, 2, 3]
+  the output list would also be
+    [1, 2, 3].
 */
 
-function calc_seconds(
-  seconds: int, minutes: int, hours: int, days: int
-): int
-{
-  86400 * days + 3600 * hours + 60 * minutes + seconds
-}
-
-function stopwatch_invariant(
-  seconds: int, minutes: int, hours: int, days: int
-): bool
-{
-  0 <= seconds < 60 && 0 <= minutes < 60 && 0 <= hours < 24 && days >= 0
-}
-
-method AdvanceStopwatch(
-  seconds: int, minutes: int, hours: int, days: int,
-  advance_by: int
-) returns (new_seconds: int, new_minutes: int, new_hours: int, new_days: int)
-  requires stopwatch_invariant(seconds, minutes, hours, days)
-  ensures stopwatch_invariant(new_seconds, new_minutes, new_hours, new_days)
-  ensures calc_seconds(new_seconds, new_minutes, new_hours, new_days)
-       == calc_seconds(seconds, minutes, hours, days) + advance_by
+method CopySequence(a: seq<int>) returns (b: seq<int>)
+  ensures |b| == |a|
+  ensures forall i :: 0 <= i < |a| ==> a[i] == b[i]
   // TODO: delete the following line and implement the function
   requires false
 {
@@ -103,8 +88,78 @@ method AdvanceStopwatch(
 }
 
 /*
-  4. Uncomment the following tests to make sure that
+  4. List partial sum
+
+  Compute the partial sums of a list. For example, if the
+  input list is
+    [1, 2, 3]
+  the output list would be
+    [0, 1, 3, 6].
+
+  Note: It doesn't sound tricky, but this one is hard!
+  You may need to use a lemma to get the verification to pass.
+
+  We have provided a space for a helper lemma below and
+  a brief explanation of how lemmas work.
+  Check out the hints.md file if you get stuck!
+
+  ===== What are lemmas? =====
+
+  A lemma is written as a method that provides
+  an additional postcondition. A lemma may or may not have a body.
+  You can write one like this:
+
+  method Lemma(a: seq<int>)
+    ensures <some conditions>
+  {
+  }
+
+  To call the lemma, you just call the method.
+  It brings the postcondition assert in scope so that Dafny
+  can use it to verify the code in the location you're working on.
+
+    // Call the lemma
+    Lemma();
+    // Prove some additional assertions that were failing using the lemma
+    assert <some hard condition>;
+
+*/
+
+// This function is needed to state the pre/postconditions
+function array_sum(a: seq<int>): int
+{
+  if |a| == 0 then 0 else (a[|a| - 1] + array_sum(a[..(|a| - 1)]))
+}
+
+// Space for lemmas
+lemma Lemma1(a: seq<int>)
+{
+  // Fill in here
+}
+lemma Lemma2(a: seq<int>)
+{
+  // Fill in here
+}
+
+method PartialSums(a: seq<int>) returns (b: seq<int>)
+  ensures |b| == |a| + 1
+  ensures forall i :: 0 <= i <= |a| ==> b[i] == array_sum(a[..i])
+  // TODO: delete the following line and implement the function
+  requires false
+{
+  // TODO
+}
+
+/*
+  5. Uncomment the following tests to make sure that
   your implementations above are working.
+
+  Note: since we've already proven the code correct,
+  using tests is not strictly necessary. You could argue
+  it's redundant.
+  The main point of this part is to make sure that you have
+  removed the `requires false` lines and implemented the methods
+  so that calling the tests actually works.
 */
 
 method Tests()
@@ -121,6 +176,11 @@ method Tests()
   // assert y1 == 3;
   // assert y2 == 1;
 
-  // var s, m, h, d := AdvanceStopwatch(0, 0, 0, 0, 65);
-  // assert s == 5 && m == 1 && h == 0 && d == 0;
+  // var a1 := [1, 2, 3];
+  // var b1 := CopySequence(a1);
+  // assert a1 == b1;
+
+  // var a2 := [1, 2, 3];
+  // var b2 := PartialSums(a2);
+  // assert b2 == [0, 1, 3, 6];
 }
